\documentclass[fleqn, a4paper, 11pt, oneside]{amsart}
\usepackage{exsheets}
\usepackage{amsmath, amssymb, amsthm} %standard AMS packages
\usepackage{marginnote} %marginnotes
\usepackage{gensymb} %miscellaneous symbols
\usepackage{commath} %differential symbols
\usepackage{xcolor} %colours
\usepackage{cancel} %cancelling terms
\usepackage[free-standing-units, space-before-unit]{siunitx} %formatting units
\usepackage{tikz, pgfplots} %diagrams
	\usetikzlibrary{calc, hobby, patterns, intersections, decorations.markings}
\usepackage{graphicx} %inserting graphics
\usepackage{hyperref} %hyperlinks
\usepackage{datetime} %date and time
\usepackage{enumerate,enumitem} %numbered lists
\usepackage{float} %inserting floats
\usepackage{circuitikz}[american voltages, american currents] %circuit diagrams

\newcommand\numberthis{\addtocounter{equation}{1}\tag{\theequation}} %adds numbers to specific equations in non-numbered list of equations

\theoremstyle{definition}
\newtheorem{example}{Example}
\newtheorem{definition}{Definition}

\theoremstyle{theorem}
\newtheorem{theorem}{Theorem}

\makeatletter
\@addtoreset{section}{part} %resets section numbers in new part
\makeatother

\SetupExSheets{solution/print = true}

%opening
\title
[
	PDE : Assignent 1
]
{
	Partial Differential Equations\\
	Assignment 1
}
\author
{
	Aakash Jog\\
	ID : 989323563
}
\date{\formatdate{3}{3}{2016}}

\begin{document}

\maketitle
%\setlength{\mathindent}{0pt}

\begin{question}
	Solve
	\begin{align*}
		u_{t t}  & = u_{x x}           \\
		u(x,0)   & = \frac{x}{1 + x^2} \\
		u_t(x,0) & = \sin x
	\end{align*}
	where $-\infty < x < \infty$, and $t > 0$.
\end{question}

\begin{solution}
	Comparing to the standard form,
	\begin{align*}
		a    & = 1                 \\
		f(x) & = \frac{x}{1 + x^2} \\
		g(x) & = \sin x
	\end{align*}
	Therefore, by the d'Alembert formula,
	\begin{align*}
		u(x,t) & = \frac{f(x - a t) + f(x + a t)}{2} + \frac{1}{2 a} \int\limits_{x - a t}^{x + a t} g(s) \dif s                                                  \\
                       & = \frac{f(x - t) + f(x + t)}{2} + \frac{1}{2} \int\limits_{x - t}^{x + t} g(s) \dif s                                                            \\
                       & = \frac{\frac{x - t}{1 + (x - t)^2} + \frac{x + t}{1 + (x + t)^2}}{2} + \frac{1}{2} \int\limits_{x - t}^{x + t} \sin s \dif s                    \\
                       & = \frac{\frac{x - t}{1 + (x - t)^2} + \frac{x + t}{1 + (x + t)^2}}{2} + \frac{1}{2} \left. \left( -\cos s \dif s \right) \right|_{x - t}^{x + t} \\
                       & = \frac{\frac{x - t}{1 + (x - t)^2} + \frac{x + t}{1 + (x + t)^2}}{2} + \frac{1}{2} \left( -\cos(x + t) + \cos(x - t) \right)                    \\
                       & = \frac{1}{2} \left( \frac{x - t}{1 + (x - t)^2} + \frac{x + t}{1 + (x + t)^2} \right) + \sin x \sin t
	\end{align*}
\end{solution}

\begin{question}
	Solve the problem and sketch the solution for different time segments.
	\begin{align*}
		u_{t t} &= 3 u_{x x}\\
		u(x,0) &=
			\begin{cases}
				1 & ;\quad 1 \le x \le 2    \\
				0 & ;\quad \text{otherwise} \\
			\end{cases}\\
		u_t(x,0) &= 0
	\end{align*}
\end{question}

\begin{solution}
	Comparing to the standard form,
	\begin{align*}
		a &= 2\\
		f(x) &=
			\begin{cases}
				1 & ;\quad 1 \le x \le 2    \\
				0 & ;\quad \text{otherwise} \\
			\end{cases}\\
		g(x) &= 0
	\end{align*}
	Therefore, by the d'Alembert formula,
	\begin{align*}
		u(x,t) & = \frac{f(x - a t) + f(x + a t)}{2} + \frac{1}{2 a} \int\limits_{x - a t}^{x + a t} g(s) \dif s \\
                       & = \frac{f(x - 2 t) + f(x + 2 t)}{2} + \frac{1}{4} \int\limits_{x - 2 t}^{x + 2 t} 0 \dif s      \\
                       & = \frac{1}{2} \left( f(x - 2 t) + f(x + 2 t) \right)
	\end{align*}
	Therefore,
	\begin{align*}
		f(x - 2 t) &=
			\begin{cases}
				1 & ;\quad 1 \le x - 2 t \le 2 \\
				0 & ;\quad \text{otherwise}    \\
			\end{cases}\\
		&=
			\begin{cases}
				1 & ;\quad 1 + 2 t \le x \le 2 + 2 t \\
				0 & ;\quad \text{otherwise}          \\
			\end{cases}\\
		f(x + 2 t) &=
			\begin{cases}
				1 & ;\quad 1 \le x + 2 t \le 2 \\
				0 & ;\quad \text{otherwise}    \\
			\end{cases}\\
		&=
			\begin{cases}
				1 & ;\quad 1 - 2 t \le x \le 2 - 2 t \\
				0 & ;\quad \text{otherwise}          \\
			\end{cases}
	\end{align*}
	For $t = 0$,
	\begin{align*}
		u(x,t) &= u(x,0)\\
		&= \frac{1}{2} \left( f(x) + f(x) \right)\\
		&= f(x)\\
		&=
			\begin{cases}
				1 & ;\quad 1 \le x \le 2    \\
				0 & ;\quad \text{otherwise} \\
			\end{cases}
	\end{align*}
	\begin{figure}[H]
		\centering
		\begin{tikzpicture}[scale = 2.5]
			\def\xMIN{-1};
			\def\xMAX{3};
			\def\yMIN{-2};
			\def\yMAX{2};
			\def\t{0};

			\begin{scope}[stealth-stealth, gray]
				\draw (\xMIN,0) -- (\xMAX,0) node [right] {$x$};
				\draw (0,\yMIN) -- (0,\yMAX) node [above] {$u(x)$};
			\end{scope}

			\begin{scope}
				\draw (\xMIN,0) -- ({1 - 2 * \t},0);
				\draw ({1 - 2 * \t},1/2) -- ({1 + 2 * \t},1/2);
				\draw ({1 + 2 * \t},1) -- ({2 - 2 * \t},1);
				\draw ({2 - 2 * \t},1/2) -- ({2 + 2 * \t},1/2);
				\draw ({2 + 2 * \t},0) -- (\xMAX,0);
			\end{scope}

			\begin{scope}[dashed]
				\draw ({1 - 2 * \t},\yMIN) -- ({1 - 2 * \t},\yMAX);
				\node [below, fill = white] at ({1 - 2 * \t},0) {$1$};
				\draw ({1 + 2 * \t},\yMIN) -- ({1 + 2 * \t},\yMAX);
				\node [below, fill = white] at ({1 + 2 * \t},0) {$1$};
				\draw ({2 - 2 * \t},\yMIN) -- ({2 - 2 * \t},\yMAX);
				\node [below, fill = white] at ({2 - 2 * \t},0) {$2$};
			\end{scope}
		\end{tikzpicture}
	\end{figure}
	\begin{figure}[H]
		\centering
		\begin{tikzpicture}[scale = 2.5]
			\def\xMIN{-1};
			\def\xMAX{3};
			\def\yMIN{-2};
			\def\yMAX{2};
			\def\t{1/8};

			\begin{scope}[stealth-stealth, gray]
				\draw (\xMIN,0) -- (\xMAX,0) node [right] {$x$};
				\draw (0,\yMIN) -- (0,\yMAX) node [above] {$u(x + 2 t)$};
			\end{scope}

			\begin{scope}
				\draw (\xMIN,0) -- ({1 - 2 * \t},0);
				\draw ({1 - 2 * \t},1/2) -- ({1 + 2 * \t},1/2);
				\draw ({1 + 2 * \t},0) -- ({2 - 2 * \t},0);
				\draw ({2 - 2 * \t},1/2) -- ({2 + 2 * \t},1/2);
				\draw ({2 + 2 * \t},0) -- (\xMAX,0);
			\end{scope}

			\begin{scope}[dashed]
				\draw ({1 - 2 * \t},\yMIN) -- ({1 - 2 * \t},\yMAX);
				\node [below, fill = white] at ({1 - 2 * \t},0) {$1 - 2 t$};
				\draw ({1 + 2 * \t},\yMIN) -- ({1 + 2 * \t},\yMAX);
				\node [below, fill = white] at ({1 + 2 * \t},0) {$1 + 2 t$};
				\draw ({2 - 2 * \t},\yMIN) -- ({2 - 2 * \t},\yMAX);
				\node [below, fill = white] at ({2 - 2 * \t},0) {$2 - 2 t$};
				\draw ({2 + 2 * \t},\yMIN) -- ({2 + 2 * \t},\yMAX);
				\node [below, fill = white] at ({2 + 2 * \t},0) {$2 + 2 t$};
			\end{scope}
		\end{tikzpicture}
	\end{figure}
	\begin{figure}[H]
		\centering
		\begin{tikzpicture}[scale = 2.5]
			\def\xMIN{-1};
			\def\xMAX{3};
			\def\yMIN{-2};
			\def\yMAX{2};
			\def\t{1/4};

			\begin{scope}[stealth-stealth, gray]
				\draw (\xMIN,0) -- (\xMAX,0) node [right] {$x$};
				\draw (0,\yMIN) -- (0,\yMAX) node [above] {$u(x + \frac{1}{2})$};
			\end{scope}

			\begin{scope}
				\draw (\xMIN,0) -- ({1 - 2 * \t},0);
				\draw ({1 - 2 * \t},1/2) -- ({1 + 2 * \t},1/2);
				\draw ({1 + 2 * \t},1) -- ({2 - 2 * \t},1);
				\draw ({2 - 2 * \t},1/2) -- ({2 + 2 * \t},1/2);
				\draw ({2 + 2 * \t},0) -- (\xMAX,0);
			\end{scope}

			\begin{scope}[dashed]
				\draw ({1 - 2 * \t},\yMIN) -- ({1 - 2 * \t},\yMAX);
				\node [below, fill = white] at ({1 - 2 * \t},0) {$\frac{1}{2}$};
				\draw ({1 + 2 * \t},\yMIN) -- ({1 + 2 * \t},\yMAX);
				\node [below, fill = white] at ({1 + 2 * \t},0) {$\frac{3}{2}$};
				\draw ({2 - 2 * \t},\yMIN) -- ({2 - 2 * \t},\yMAX);
				\node [below, fill = white] at ({2 - 2 * \t},0) {$\frac{3}{2}$};
				\draw ({2 + 2 * \t},\yMIN) -- ({2 + 2 * \t},\yMAX);
				\node [below, fill = white] at ({2 + 2 * \t},0) {$\frac{5}{2}$};
			\end{scope}
		\end{tikzpicture}
	\end{figure}
	\begin{figure}[H]
		\centering
		\begin{tikzpicture}[scale = 2.5]
			\def\xMIN{-1};
			\def\xMAX{3};
			\def\yMIN{-2};
			\def\yMAX{2};
			\def\t{1/2};

			\begin{scope}[stealth-stealth, gray]
				\draw (\xMIN,0) -- (\xMAX,0) node [right] {$x$};
				\draw (0,\yMIN) -- (0,\yMAX) node [above] {$u(x + 2 t)$};
			\end{scope}

			\begin{scope}
				\draw (\xMIN,0) -- ({1 - 2 * \t},0);
				\draw ({1 - 2 * \t},1/2) -- ({2 - 2 * \t},1/2);
				\draw ({2 - 2 * \t},1) -- ({1 + 2 * \t},1);
				\draw ({1 + 2 * \t},1/2) -- ({2 + 2 * \t},1/2);
				\draw ({2 + 2 * \t},0) -- (\xMAX,0);
			\end{scope}

			\begin{scope}[dashed]
				\draw ({1 - 2 * \t},\yMIN) -- ({1 - 2 * \t},\yMAX);
				\node [below, fill = white] at ({1 - 2 * \t},0) {$1 - 2 t$};
				\draw ({1 + 2 * \t},\yMIN) -- ({1 + 2 * \t},\yMAX);
				\node [below, fill = white] at ({1 + 2 * \t},0) {$1 + 2 t$};
				\draw ({2 - 2 * \t},\yMIN) -- ({2 - 2 * \t},\yMAX);
				\node [below, fill = white] at ({2 - 2 * \t},0) {$2 - 2 t$};
				\draw ({2 + 2 * \t},\yMIN) -- ({2 + 2 * \t},\yMAX);
				\node [below, fill = white] at ({2 + 2 * \t},0) {$2 + 2 t$};
			\end{scope}
		\end{tikzpicture}
	\end{figure}
	For $0 < t < \frac{1}{4}$,
	\begin{align*}
		u(x,t) &= \frac{1}{2} \left( f(x - 2 t) + f(x + 2 t) \right)\\
		&=
			\begin{cases}
				0           & ;\quad x < 1 - 2 t               \\
				\frac{1}{2} & ;\quad 1 - 2 t < x < 1 + 2 t     \\
				1           & ;\quad 1 + 2 t \le x \le 2 - 2 t \\
				\frac{1}{2} & ;\quad 2 - 2 t < x < 2 + 2 t     \\
				0           & ;\quad 2 + 2 t < x               \\
			\end{cases}
	\end{align*}
	For $t = \frac{1}{4}$,
	\begin{align*}
		u(x,t) &= u\left( x,\frac{1}{4} \right)\\
		&=
			\begin{cases}
				0           & ;\quad x < \frac{1}{2}                 \\
				\frac{1}{2} & ;\quad \frac{1}{2} \le x < \frac{3}{2} \\
				1           & ;\quad x = \frac{3}{2}                 \\
				\frac{1}{2} & ;\quad \frac{3}{2} < x \le \frac{5}{2} \\
				0           & ;\quad \frac{5}{2} < x                 \\
			\end{cases}
	\end{align*}
	For $\frac{1}{4} < t$,
	\begin{align*}
		u(x,t) &= \frac{1}{2} \left( f(x - 2 t) + f(x + 2 t) \right)\\
		&=
			\begin{cases}
				0           & ;\quad x < 1 - 2 t               \\
				\frac{1}{2} & ;\quad 1 - 2 t \le x \le 1 + 2 t \\
				0           & ;\quad 1 + 2 t < x < 2 - 2 t     \\
				\frac{1}{2} & ;\quad 2 - 2 t \le x \le 2 + 2 t \\
				0           & ;\quad 2 + 2 t < x               \\
			\end{cases}
	\end{align*}
	Therefore, the graphs of the solution are
	\begin{figure}[H]
		\centering
		\begin{tikzpicture}[scale = 2.5]
			\def\xMIN{-1};
			\def\xMAX{3};
			\def\yMIN{-1};
			\def\yMAX{2};
			\def\t{0};

			\begin{scope}[stealth-stealth, gray]
				\draw (\xMIN,0) -- (\xMAX,0) node [right] {$x$};
				\draw (0,\yMIN) -- (0,\yMAX) node [above] {$u(x + 2 t)$};
			\end{scope}

			\begin{scope}
				\draw (\xMIN,0) -- ({1 - 2 * \t},0);
				\draw ({1 - 2 * \t},1/2) -- ({1 + 2 * \t},1/2);
				\draw ({1 + 2 * \t},1) -- ({2 - 2 * \t},1);
				\draw ({2 - 2 * \t},1/2) -- ({2 + 2 * \t},1/2);
				\draw ({2 + 2 * \t},0) -- (\xMAX,0);
			\end{scope}

			\begin{scope}[dashed]
				\draw ({1 - 2 * \t},\yMIN) -- ({1 - 2 * \t},\yMAX);
				\node [below, fill = white] at ({1 - 2 * \t},0) {$1$};
				\draw ({1 + 2 * \t},\yMIN) -- ({1 + 2 * \t},\yMAX);
				\node [below, fill = white] at ({1 + 2 * \t},0) {$1$};
				\draw ({2 - 2 * \t},\yMIN) -- ({2 - 2 * \t},\yMAX);
				\node [below, fill = white] at ({2 - 2 * \t},0) {$2$};
			\end{scope}
		\end{tikzpicture}
		\caption{$t = 0$}
	\end{figure}
	\begin{figure}[H]
		\centering
		\begin{tikzpicture}[scale = 2.5]
			\def\xMIN{-1};
			\def\xMAX{3};
			\def\yMIN{-1};
			\def\yMAX{2};
			\def\t{1/8};

			\begin{scope}[stealth-stealth, gray]
				\draw (\xMIN,0) -- (\xMAX,0) node [right] {$x$};
				\draw (0,\yMIN) -- (0,\yMAX) node [above] {$u(x + 2 t)$};
			\end{scope}

			\begin{scope}
				\draw (\xMIN,0) -- ({1 - 2 * \t},0);
				\draw ({1 - 2 * \t},1/2) -- ({1 + 2 * \t},1/2);
				\draw ({1 + 2 * \t},0) -- ({2 - 2 * \t},0);
				\draw ({2 - 2 * \t},1/2) -- ({2 + 2 * \t},1/2);
				\draw ({2 + 2 * \t},0) -- (\xMAX,0);
			\end{scope}

			\begin{scope}[dashed]
				\draw ({1 - 2 * \t},\yMIN) -- ({1 - 2 * \t},\yMAX);
				\node [below, fill = white] at ({1 - 2 * \t},0) {$1 - 2 t$};
				\draw ({1 + 2 * \t},\yMIN) -- ({1 + 2 * \t},\yMAX);
				\node [below, fill = white] at ({1 + 2 * \t},0) {$1 + 2 t$};
				\draw ({2 - 2 * \t},\yMIN) -- ({2 - 2 * \t},\yMAX);
				\node [below, fill = white] at ({2 - 2 * \t},0) {$2 - 2 t$};
				\draw ({2 + 2 * \t},\yMIN) -- ({2 + 2 * \t},\yMAX);
				\node [below, fill = white] at ({2 + 2 * \t},0) {$2 + 2 t$};
			\end{scope}
		\end{tikzpicture}
		\caption{$0 < t < \frac{1}{4}$}
	\end{figure}
	\begin{figure}[H]
		\centering
		\begin{tikzpicture}[scale = 2.5]
			\def\xMIN{-1};
			\def\xMAX{3};
			\def\yMIN{-1};
			\def\yMAX{2};
			\def\t{1/4};

			\begin{scope}[stealth-stealth, gray]
				\draw (\xMIN,0) -- (\xMAX,0) node [right] {$x$};
				\draw (0,\yMIN) -- (0,\yMAX) node [above] {$u(x + 2 t)$};
			\end{scope}

			\begin{scope}
				\draw (\xMIN,0) -- ({1 - 2 * \t},0);
				\draw ({1 - 2 * \t},1/2) -- ({1 + 2 * \t},1/2);
				\draw ({1 + 2 * \t},1) -- ({2 - 2 * \t},1);
				\draw ({2 - 2 * \t},1/2) -- ({2 + 2 * \t},1/2);
				\draw ({2 + 2 * \t},0) -- (\xMAX,0);
			\end{scope}

			\begin{scope}[dashed]
				\draw ({1 - 2 * \t},\yMIN) -- ({1 - 2 * \t},\yMAX);
				\node [below, fill = white] at ({1 - 2 * \t},0) {$\frac{1}{2}$};
				\draw ({1 + 2 * \t},\yMIN) -- ({1 + 2 * \t},\yMAX);
				\node [below, fill = white] at ({1 + 2 * \t},0) {$\frac{3}{2}$};
				\draw ({2 - 2 * \t},\yMIN) -- ({2 - 2 * \t},\yMAX);
				\node [below, fill = white] at ({2 - 2 * \t},0) {$\frac{3}{2}$};
				\draw ({2 + 2 * \t},\yMIN) -- ({2 + 2 * \t},\yMAX);
				\node [below, fill = white] at ({2 + 2 * \t},0) {$\frac{5}{2}$};
			\end{scope}
		\end{tikzpicture}
		\caption{$t = \frac{1}{4}$}
	\end{figure}
	\begin{figure}[H]
		\centering
		\begin{tikzpicture}[scale = 2.5]
			\def\xMIN{-1};
			\def\xMAX{3};
			\def\yMIN{-1};
			\def\yMAX{2};
			\def\t{1/2};

			\begin{scope}[stealth-stealth, gray]
				\draw (\xMIN,0) -- (\xMAX,0) node [right] {$x$};
				\draw (0,\yMIN) -- (0,\yMAX) node [above] {$u(x + 2 t)$};
			\end{scope}

			\begin{scope}
				\draw (\xMIN,0) -- ({1 - 2 * \t},0);
				\draw ({1 - 2 * \t},1/2) -- ({2 - 2 * \t},1/2);
				\draw ({2 - 2 * \t},1) -- ({1 + 2 * \t},1);
				\draw ({1 + 2 * \t},1/2) -- ({2 + 2 * \t},1/2);
				\draw ({2 + 2 * \t},0) -- (\xMAX,0);
			\end{scope}

			\begin{scope}[dashed]
				\draw ({1 - 2 * \t},\yMIN) -- ({1 - 2 * \t},\yMAX);
				\node [below, fill = white] at ({1 - 2 * \t},0) {$1 - 2 t$};
				\draw ({1 + 2 * \t},\yMIN) -- ({1 + 2 * \t},\yMAX);
				\node [below, fill = white] at ({1 + 2 * \t},0) {$1 + 2 t$};
				\draw ({2 - 2 * \t},\yMIN) -- ({2 - 2 * \t},\yMAX);
				\node [below, fill = white] at ({2 - 2 * \t},0) {$2 - 2 t$};
				\draw ({2 + 2 * \t},\yMIN) -- ({2 + 2 * \t},\yMAX);
				\node [below, fill = white] at ({2 + 2 * \t},0) {$2 + 2 t$};
			\end{scope}
		\end{tikzpicture}
		\caption{$\frac{1}{4} < t$}
	\end{figure}
\end{solution}

\begin{question}
	Solve
	\begin{enumerate}
		\item
			\begin{align*}
				u_{t t} &= u_{x x}\\
				u(x,0) &=
					\begin{cases}
						\sin x  & ;\quad x \ge 0 \\
						-\sin x & ;\quad x < 0   \\
					\end{cases}\\
				u_t(x,0) &= -\cos x
			\end{align*}
			where $-\infty < x < \infty$, and $t > 0$.
		\item
			\begin{align*}
				u_{t t} &= u_{x x}\\
				u(x,0) &= -\cos x\\
				u_t(x,0) &=
					\begin{cases}
						\sin x  & ;\quad x \ge 0 \\
						-\sin x & ;\quad x < 0   \\
					\end{cases}
			\end{align*}
			where $-\infty < x < \infty$, and $t > 0$.
	\end{enumerate}
\end{question}

\begin{solution}
	\begin{enumerate}[leftmargin=*]
		\item
			Comparing to the standard form,
			\begin{align*}
				a &= 1\\
				f(x) &=
					\begin{cases}
						\sin x  & ;\quad x \ge 0 \\
						-\sin x & ;\quad x < 0   \\
					\end{cases}\\
				g(x) &= -\cos x
			\end{align*}
			Therefore, by the d'Alembert formula,
			\begin{align*}
				u(x,t) &= \frac{f(x - a t) + f(x + a t)}{2} + \frac{1}{2 a} \int\limits_{x - a t}^{x + a t} g(s) \dif s\\
				&= \frac{f(x - t) + f(x + t)}{2} + \frac{1}{2} \int\limits_{x - t}^{x + t} (-\cos s) \dif s\\
				&= \frac{f(x - t) + f(x + t)}{2} + \frac{1}{2} \left( \sin(x - t) - \sin(x + t) \right)\\
				&=
					\begin{cases}
						\frac{1}{2} \left( \sin(x - t) + \sin(x + t) \right) + \frac{1}{2} \left( \sin(x - t) - \sin(x + t) \right)  & ;\quad x \ge 0 \\
						\frac{1}{2} \left( -\sin(x - t) - \sin(x + t) \right) + \frac{1}{2} \left( \sin(x - t) - \sin(x + t) \right) & ;\quad x < 0   \\
					\end{cases}\\
				&=
					\begin{cases}
						\sin(x - t)  & ;\quad x \ge 0 \\
						-\sin(x + t) & ;\quad x < 0   \\
					\end{cases}
			\end{align*}
		\item
			Comparing to the standard form,
			\begin{align*}
				a &= 1\\
				f(x) &= -\cos x\\
				g(x) &=
					\begin{cases}
						\sin x  & ;\quad x \ge 0 \\
						-\sin x & ;\quad x < 0   \\
					\end{cases}
			\end{align*}
			Therefore, by the d'Alembert formula,
			\begin{align*}
				u(x,t) &= \frac{f(x - a t) + f(x + a t)}{2} + \frac{1}{2 a} \int\limits_{x - a t}^{x + a t} g(s) \dif s\\
				&= \frac{-\cos(x - t) - \cos(x + t)}{2} + \frac{1}{2} \int\limits_{x - t}^{x + t} g(s) \dif s\\
				&= \quad \frac{-\cos(x - t) - \cos(x + t)}{2}\\
				&\quad +
					\begin{cases}
						\frac{1}{2} \int\limits_{x - t}^{x + t} \sin(s) \dif s                                                      & ;\quad x \ge t \\
						\frac{1}{2} \left( \int\limits_{x - t}^{0} -\sin(s) \dif s + \int\limits_{0}^{x + t} \sin(s) \dif s \right) & ;\quad x < t   \\
					\end{cases}\\
				&= \quad \frac{-\cos(x - t) - \cos(x + t)}{2}\\
				&\quad +
					\begin{cases}
						\frac{1}{2} \left( -\cos(x + t) + \cos(x - t) \right)                                                   & ;\quad x \ge t \\
						\frac{1}{2} \left( \left( \cos(0) - \cos(x - t) \right) + \left( -\cos(x + t) + \cos(0) \right) \right) & ;\quad x < t   \\
					\end{cases}\\
				&= \quad \frac{-\cos(x - t) - \cos(x + t)}{2}\\
				&\quad +
					\begin{cases}
						-\cos(x - t)                  & ;\quad x \ge t \\
						1 - \cos(x - t) - \cos(x + t) & ;\quad x < t   \\
					\end{cases}
			\end{align*}
	\end{enumerate}
\end{solution}

\end{document}
